{
 "cells": [
  {
   "cell_type": "markdown",
   "metadata": {},
   "source": [
    "# Lecture 03 - 20 September 2021\n",
    "\n",
    "Equipped with the definitions and lemmas found in the last lecture it is possible to start talking about the **z-transform**. But first, it is necessary to draw some parallelisms with the solutions of a differential equation:\n",
    "\n",
    "![Solution of a differential equation with Fourier Transform / Laplace Transform](images/21-09-20_diff_eq_sol.png)\n",
    "  \n",
    "  \n",
    "  \n",
    "For example, with a low pass filter, the procedure becomes:  \n",
    "![Solution of the low pass with Fourier Tranform](images/21-09-20_diff_eq_example.png)\n",
    "\n",
    "  \n",
    "  \n",
    "Similarly, a difference equation can be solved via an appropriate transform, the z-transform\n",
    "![Solution of a difference equation with z-transform](images/21-09-20_z-transform_sol.png)\n",
    "\n",
    "## The z-transform\n",
    "Given a sequence $x[n]$ we write the z-transform as\n",
    "\\begin{align*}\n",
    "    Z\\left(x[n]\\right) = X(z) = \\sum_{\\forall n} z^{-n} x[n] \\qquad \\text{ with } \\qquad z \\in \\textbf{R.O.C} \\subseteq \\mathcal{C}.\n",
    "\\end{align*}\n",
    "In the previous definition **R.O.C** stands for _Region Of Convergence_, the region of the complex plane where the series converges to a finite value.\n",
    "  \n",
    "Some remarkable examples of z-tranforms are:\n",
    "\n",
    "### The delta\n",
    "\\begin{align*}\n",
    "    Z\\left(\\delta[n]\\right) = \\sum_{n=-\\infty}^{+\\infty} z^{-n} \\delta[n] = 1 \\qquad \\textbf{R.O.C} = \\mathcal{C}\n",
    "\\end{align*}\n",
    "\n",
    "### Step sequence\n",
    "\\begin{align*}\n",
    "   Z\\left(U[n]\\right) &= \\sum_{n=-\\infty}^{+\\infty} z^{-n} U[n] = \\sum_{n=0}^{+\\infty} z^{-n} = \\frac{1}{1-1/z} = \\frac{z}{z-1}  \\\\\n",
    "   \\text{ROC} &= \\left\\{ z : \\frac{1}{|z|} < 1 \\implies |z|>1\\right\\}\n",
    "\\end{align*}\n",
    "\n",
    "### Step sequence (second case)\n",
    "\\begin{align*}\n",
    "    Z\\left(-U[-n-1]\\right) &= -\\sum_{n=-\\infty}^{+\\infty} z^{-n} U[-n-1] = - \\sum_{n=1}^{+\\infty} z^{n} = 1- \\frac{1}{1-z} = \\frac{z}{z-1} \\\\\n",
    "    \\text{ROC} &= \\left\\{ z : \\frac{1}{|z|} > 1 \\implies |z|<1\\right\\}\n",
    "\\end{align*}\n",
    "\n",
    "It is possible to notice that two different functions led to the same z-transform but different R.O.C. A warning is due:\n",
    "\n",
    "```{warning}\n",
    "The z-transform is NOT sufficient to characterize a system in the z domain. The R.O.C. is part of the system too!\n",
    "```\n",
    "\n",
    "## Properties of the z-transform\n",
    "\n",
    "Let $X[z] = Z(x[n])$\n",
    "\n",
    "### Time shift\n",
    "\\begin{align*}\n",
    "    Z\\left(x[n-n_0]\\right) = \\sum_{n=-\\infty}^{+\\infty} z^{-n} x[n-n_0] = \\sum_{n=-\\infty}^{+\\infty} z^{-(n-n_0)} z^{-n_0} x[n-n_0] = z^{-n_0} X(z)\n",
    "\\end{align*}\n",
    "\n",
    "### Linearity\n",
    "\\begin{align*}\n",
    "    Z\\left(a x[n] + b y[n]\\right) &= \\sum_{n=-\\infty}^{+\\infty} z^{-n} (ax[n]+by[n]) = a X(z) + b X(z) \\\\\n",
    "    \\text{ROC} &= \\textbf{R.O.C}_x \\cap \\textbf{R.O.C}_y\n",
    "\\end{align*}\n",
    "\n",
    "### Convolution\n",
    "\\begin{align*}\n",
    "    Z\\left(x[n]*y[n]\\right) &= Z\\left(\\sum_k x[n-k]y[k] \\right) = \\sum_{k=-\\infty}^{+\\infty} Z(x[n-k])y[k] \\\\\n",
    "    &= \\sum_{k=-\\infty}^{+\\infty} Z(x[n])z^{-k}y[k] = X(z) Y(z) \\\\\n",
    "    \\text{ROC} &= \\textbf{R.O.C}_x \\cap \\textbf{R.O.C}_y\n",
    "\\end{align*}\n",
    "\n",
    "### Cascade of two systems\n",
    "![Cascade of two systems](images/21-09-20_cascade_of_two_systems.png)\n",
    "\n",
    "If the two systems are L.T.I. the two cascade are equivalent: $y[n]=y'[n]$. The proof lies in the equality of the z-transform and the properties of the convolution. More than that, the two systems $y[n]$ and $y'[n]$ have the same R.O.C:\n",
    "  \n",
    "\\begin{align*}\n",
    "    y[n] &= h[n]*j[n] = Z^{-1}\\left(h(z)j(z)\\right) = Z^{-1}\\left(j(z)h(z)\\right) = j[n]*h[n] = y'[n] \\\\\n",
    "    \\text{ROC} &= \\text{ROC}_x \\cap \\text{ROC}_y\n",
    "\\end{align*}\n",
    "    \n",
    "In the last properties, the notion of inverse z-transform was suggested. To give a formal definition of inverse z-transform some lemmas are needed.\n",
    "\n",
    "## Lemmas for inverse z-transform\n",
    "\n",
    "### Close path integral\n",
    "The close path integral around (**um**) a single pole  $z_0$ depends only on the order of the pole:\n",
    "\\begin{align*}\n",
    "    \\frac{1}{2\\pi i} \\oint_{\\Gamma\\text{ um }z_0} (z-z_0)^n dz = \\delta_{n, -1} \\qquad \\text{ with } n \\in \\mathcal{Z}\n",
    "\\end{align*}\n",
    "\n",
    "**proof**  \n",
    "Take a circle of radius $r$ around $z_0$ such that $z=z_0+re^{i\\phi}$. Then:\n",
    "\\begin{align*}\n",
    "    \\frac{1}{2\\pi i} \\oint_{\\Gamma\\text{ um }z_0} r^n e^{i\\phi n} r e^{i\\phi} i d\\phi = \\frac{r^{n+1}}{2\\pi}\\int_{0}^{2\\pi} e^{i\\phi (n+1)} d\\phi = \\begin{cases}\n",
    "  1 \\qquad \\text{if } n=-1\\\\\n",
    "  0 \\qquad \\text{otherwise}\n",
    "\\end{cases}\n",
    "\\end{align*}\n",
    "\n",
    "I like to call this lemma the \"hidden logarithm lemma\" because it reminds me of the integral $\\int x^n dx$. For every value of $n$ the integral $\\int x^n dx$ remains a rational function, except when $n=-1$ like in this case.\n",
    "\n",
    "### Residual theorem\n",
    "\\begin{align*}\n",
    "    \\frac{1}{2\\pi i} \\oint_{\\Gamma\\text{ um }z_0} G(z) dz = \\frac{1}{(n-1)!} \\left[ \\frac{d^{n-1}}{dz^{n-1}} G(z)(z-z_0)^n \\right]_{z=z_0} \\qquad \\text{ with } n \\in \\mathcal{Z}\n",
    "\\end{align*}\n",
    "\n",
    "**proof**  \n",
    "Let's consider a function $H(z)=G(z)(z-z_0)^n$ which has NO POLES ($\\implies$ it is analytic). By writing its [Laurent series](https://en.wikipedia.org/wiki/Laurent_series) one obtains:\n",
    "\\begin{align*}\n",
    "H(z)&=G(z)(z-z_0)^n = \\sum_{k=0}^{+\\infty} \\frac{(z-z_0)^k}{k!} \\left[ \\frac{d^k}{dz^k} H(z)\\right]_{z=z_0}\\\\\n",
    "\\implies& G(z) = \\sum_{k=0}^{+\\infty} \\frac{(z-z_0)^{k-n}}{k!} \\left[ \\frac{d^k}{dz^k} H(z)\\right]_{z=z_0}\n",
    "\\end{align*}\n",
    "\n",
    "By computing the integral using the previous lemma:\n",
    "\\begin{align*}\n",
    "     \\frac{1}{2\\pi i} \\oint_{\\Gamma\\text{ um }z_0} G(z) dz &= \\sum_{k=0}^{\\infty}\\frac{1}{k!} \\left[ \\frac{d^k}{dz^k}H(z)\\right]_{z=z_0}\\cdot \\frac{1}{2\\pi i} \\oint_{\\Gamma\\text{ um }z_0} (z-z_0)^n dz \\\\\n",
    "     &= \\frac{1}{(n-1)!}\\left[ \\frac{d^{n-1}}{dz^{n-1}} G(z)(z-z_0)^n \\right]_{z=z_0}\n",
    "\\end{align*}\n",
    "\n",
    "### Inversion of the z-transform\n",
    "If $X(z)=Z(x[n])$ then $x[n]=\\frac{1}{2\\pi i} \\oint_{\\Gamma\\text{ um }z_0} X(z) z^{n-1} dz$\n",
    "\n",
    "**proof**  \n",
    "\\begin{align*}\n",
    "    \\frac{1}{2\\pi i} \\oint_{\\Gamma\\text{ um }z_0} X(z)z^{n-1} dz &= \\frac{1}{2\\pi i} \\oint_{\\Gamma\\text{ um }z_0} \\sum_{k}x[k]z^{-k}z^{n-1} dz \\\\\n",
    "    &= \\frac{1}{2\\pi i} \\sum_{k} x[k] \\oint_{\\Gamma\\text{ um }z_0} z^{n-k-1} dz \\\\\n",
    "    &= \\sum_{k}x[k] \\delta_{n-k-1, -1} = x[n]\n",
    "\\end{align*}\n",
    "where the second equality assumes the R.O.C. to be such that the inversion of the summation and the integral is possible."
   ]
  }
 ],
 "metadata": {
  "kernelspec": {
   "display_name": "Python 3 (ipykernel)",
   "language": "python",
   "name": "python3"
  },
  "language_info": {
   "codemirror_mode": {
    "name": "ipython",
    "version": 3
   },
   "file_extension": ".py",
   "mimetype": "text/x-python",
   "name": "python",
   "nbconvert_exporter": "python",
   "pygments_lexer": "ipython3",
   "version": "3.8.10"
  },
  "widgets": {
   "application/vnd.jupyter.widget-state+json": {
    "state": {},
    "version_major": 2,
    "version_minor": 0
   }
  }
 },
 "nbformat": 4,
 "nbformat_minor": 4
}